src/Repr/Tactics/Opburn.v
@@ -1,0 +1,224 @@
+Require Import Omega.
+Require Import List.
+
+Require Import Repr.Tactics.Plugin.ConstructionTac.
+
+(* Searches for x in a left-associated list of nested tuples *)
+Ltac in_list ls x :=
+  match ls with
+    | x => idtac
+    | (_, x) => idtac
+    | (?ls', _) => in_list ls' x
+  end.
+
+(** Try calling tactic function [f] on all hypotheses, keeping the first application that doesn't fail. *)
+Ltac app_hyps f :=
+  match goal with
+    | [ H : _ |- _ ] => f H
+  end.
+
+(** Try calling tactic function [f] on every element of tupled list [ls], keeping the first call not to fail. *)
+Ltac app ls f :=
+  match ls with
+    | (?LS, ?X) => f X || app LS f || fail 1
+    | _ => f ls
+  end.
+
+(** Run [f] on every element of [ls], not just the first that doesn't fail. *)
+Ltac all ls f :=
+  match ls with
+    | (?LS, ?X) => f X; all LS f
+    | (_, _) => fail 1
+    | _ => f ls
+  end.
+
+(* Tactic to get rid of the manual rip/intros gen cycle *)
+Ltac loosen t :=
+  let rec gen_ls ls :=
+    match ls with
+      | false        => idtac
+      | (t,   ?ls')  => gen_ls ls'
+      | (?t', ?ls')  => generalize dependent t' ; gen_ls ls'
+    end
+  in
+
+  let rec loosen_ls ls :=
+    match goal with
+      | [ |- forall x, _ ] => 
+        intro x ;
+        loosen_ls (x,ls) 
+      | _ => gen_ls ls 
+    end
+  in
+  loosen_ls false.
+
+(* LAST : There is a tradeoff here: We want to perform as many obvious inversions
+   as possible. Easy cases where we are confident we are making the right choice.
+   (1) Inversion succeeds imediately (clears current goal)
+   (2) Inversion introduces a single constructor (simplies current goal)
+   (3) Inversion introduces multiple constructors, but they are immediately solved 
+       with eauto. *)
+Ltac simpl_hyp inv_one := 
+  (* From Chlipala: Helper tactic that inverts a hypothesis with a predicate appearing
+     in inv_one iff we immediately clear the inversion or it leaves 1 constructor *)
+  let invert_hyp F H :=
+    in_list inv_one F; 
+
+    (* Go with an attempt at quick inversion heuristics first *)
+    (inversion H; fail) || 
+    (inversion H; [idtac]; clear H; subst) ||
+
+    (* Allow an inversion if all goals are immediately solved with eauto *)
+    (inversion H; subst; solve [eauto]; clear H) ||
+
+    (* Allow an inversion if only one goal remains after euato *)
+    (inversion H; subst; eauto; [idtac]; clear H) 
+  in
+
+  match goal with
+    (* Eliminate existential hypothesis *)
+    | [ H : ex _ |- _ ] => destruct H
+
+    (* Look for any predicates that can be inverted up to a fixed arity *)
+    | [ H : ?F _ |- _ ] => invert_hyp F H
+    | [ H : ?F _ _ |- _ ] => invert_hyp F H
+    | [ H : ?F _ _ _|- _ ] => invert_hyp F H
+    | [ H : ?F _ _ _ _ |- _ ] => invert_hyp F H
+    | [ H : ?F _ _ _ _ _ |- _ ] => invert_hyp F H
+
+    (* One more trick for proof search: If we see something that intuition can
+       solve, let simpl_hyp pass *)
+    | [ H : _ \/ _ |- _ ] => idtac
+    | [ H : _ /\ _ |- _ ] => idtac
+  end.
+
+Definition done (T : Type) (x : T) := True.
+Arguments done [T] _.
+
+Definition gend (T : Type) (x : T) := True.
+Arguments gend [T] _.
+
+
+(* [e] is a universally quantified hypothesis we attemp to instantiate
+   [trace] marks the current state of our instantiation. Combine this with
+   [done] above to add state to the context. *)
+Ltac inster_prim e trace :=
+  match type of e with
+    | forall x : ?T, _ =>
+      (* One modication to the search: We generate all easy constructors for a type
+         if we haven't generated them for said type before *)
+      (match type of T with
+        | Prop => idtac
+        | _    => 
+          match goal with
+            | [ H : gend T |- _ ] => idtac
+            | _ => 
+              gen_constructors T ; 
+              assert (gend T) by constructor
+          end
+      end) ;
+
+      (* This picks the first context variable with the right type *)
+      match goal with
+        | [ H : _ |- _ ] =>
+          inster_prim (e H) (trace, H)
+        | _ => fail 2 
+      end
+    | _ =>
+      (* No more quantifiers, so we check the trace *)
+      match trace with
+        (_,_) =>
+        (* Case is only reached if trace is non-empty, forcing a fail if no 
+           progress is made *)
+        match goal with 
+          | [ H : done (trace, _) |- _ ] =>
+            (* Record of the trace in the context, backtrack *)
+            fail 1
+          | _ =>
+            let T := type of e in
+            match type of T with
+              | Prop =>
+                (* [e] is now a proof. Add it to the context and mark the trace *)
+                generalize e; intro; assert (done (trace, tt)) by constructor 
+              | _ =>
+                (* [e] is not a proof. Make sure we have not encountered this case in 
+                   the trace before proceeding. *)
+                all trace ltac:(fun X =>
+                    match goal with
+                      | [ H : done (_, X) |- _ ] => fail 1
+                      | _ => idtac
+                    end);
+                let i := fresh "i" in
+                pose (i := e); assert (done (trace, i)) by constructor
+            end
+        end
+      end
+  end.
+
+(* A Wrapper aroudn inster_prim: Before doing anything, we generate 'easy` constructors
+   of the quantified type and add them to the context *)
+(* with inster_gen e trace :=
+  match type of e with
+    | forall x : ?T, _ =>
+      (* We need to catch the implication degenerative case of product type
+         and cut off the constructor gen *)
+      match type of T with
+        | Prop => fail 1
+        | _    => gen_constructors T ; inster_prim e trace
+      end
+    | _ =>
+      inster_prim e trace
+  end. *)
+
+Ltac inster e trace :=
+  inster_prim e trace.
+  
+
+Ltac un_done :=
+  repeat match goal with
+           | [ H : done _ |- _ ] => clear H
+         end.
+
+Ltac un_gend :=
+  repeat match goal with
+           | [ H : gend _ |- _ ] => clear H
+         end.
+
+
+Ltac opburn'' lemmas inv_one guide :=
+  (* From Chlipala: Combine intuition with some simplification *)
+  let sintuition := simpl in *; intuition eauto; subst; 
+    repeat (simpl_hyp inv_one; intuition eauto; subst); try congruence in
+
+  (sintuition;
+   match lemmas with 
+     | tt => idtac
+     | _ =>
+       repeat (
+          try (app_hyps guide) ;
+          (app lemmas ltac:(fun L => inster L L) 
+           || app_hyps ltac:(fun L => inster L L)) ; 
+          repeat (simpl_hyp inv_one; intuition)
+         ) ; un_done; un_gend
+    end;
+    sintuition;
+    try omega; try (elimtype False; omega)).
+
+Ltac opburn := opburn'' tt tt ltac:(fun T => idtac).
+Ltac opburn' lemmas inv_one := opburn'' lemmas inv_one ltac:(fun T => idtac).
+
+(* Take a guess at specializing a quantified hypothesis H with v,
+   but only succeed if we can simplfy the hypothesis after specializing *)
+Ltac guess v H :=
+  let contains H :=
+    match goal with 
+      | [ _ : H |- _ ] => idtac
+      | _ => fail
+    end
+  in
+
+  specialize (H v);
+  match (type of H) with
+    | ?Head -> _ => contains Head
+    | _ => fail
+  end.
