src/Repr/Tactics/Plugin/construction.ml4
@@ -1,0 +1,49 @@
+DECLARE PLUGIN "construction_plugin"
+
+open Inductiveops
+open Pp
+
+(* Write a tactic that inspecs a type introduces all primative constructions
+   (i.e., constants) of that type into the hypothesis *)
+
+(* Making progress. In particular, we need to inspec:
+    - declarations.ml for inspecting all possible constructions of a type
+    - pre_env.ml for getting information from declarations.ml
+    - names.ml for querying the enviornment and declarations *)
+
+
+(* Ignore universe information for now *)
+
+let constrs_from_type env types =
+  let pind = Inductive.find_inductive env types in
+  let fam = Inductiveops.make_ind_family pind in
+  let constrs = Inductiveops.get_constructors env fam in
+  constrs
+
+let intro_nary_constrs constrs =
+  (* msg_info (Pp.str (Printf.sprintf "Length of constrs %d" (Array.length constrs))) ; *)
+  Array.fold_left (
+    fun m cs -> 
+      (* msg_info (Pp.str (Printf.sprintf "cs_params:%d cs_nargs:%d" (List.length cs.cs_params) cs.cs_nargs)) ; *)
+      if cs.cs_nargs == 0
+        then begin
+          let c = Inductiveops.build_dependent_constructor cs in
+          Proofview.tclTHEN (Tactics.letin_tac None Names.Anonymous c None Locusops.nowhere) m
+        end
+      else m
+  ) (Proofview.tclUNIT ()) constrs 
+  
+module ConstructionTactics = struct
+  
+  let gen_constructors types =
+    Proofview.Goal.enter ( 
+      fun gl ->
+        let constrs = constrs_from_type (Proofview.Goal.env gl) types in
+        intro_nary_constrs constrs 
+    )
+
+end 
+
+TACTIC EXTEND gen_constructors
+| ["gen_constructors" constr(c)] -> [ConstructionTactics.gen_constructors c]
+END
